Add some initial support for serialization

examples/struct/keyvalue.pos/Test.fst
@@ -157,6 +157,67 @@ let parse_abstract_store : parser store =
   (fun entries -> parsing_done `and_then`
   (fun _ -> parse_ret (Store num_entries entries))))
 
+(*! Serialization *)
+
+assume val u16_to_be: U16.t -> b:bytes{length b == 2}
+assume val u32_to_be: U32.t -> b:bytes{length b == 4}
+
+let encode_u16_array (len:U16.t) (b:bytes{length b == U16.v len}) : bytes =
+  u16_to_be len `append` b
+
+let encode_u32_array (len:U32.t) (b:bytes{length b == U32.v len}) : bytes =
+  u32_to_be len `append` b
+
+val encode_entry: encoded_entry -> bytes
+let encode_entry e = encode_u16_array e.key_len e.key `append` encode_u32_array e.val_len e.value
+
+assume val u16_be_inv: n:U16.t -> Lemma (u16_from_be (u16_to_be n) == n)
+                                 [SMTPat (u16_from_be (u16_to_be n))]
+assume val u32_be_inv: n:U32.t -> Lemma (u32_from_be (u32_to_be n) == n)
+                                 [SMTPat (u32_from_be (u32_to_be n))]
+
+
+val slice_append_suffix: #a:Type -> s1:seq a -> s2:seq a ->
+  n1:nat{n1 == length s1} -> n2:nat{n2 == length (append s1 s2)} ->
+  Lemma (slice (append s1 s2) n1 n2 == s2)
+  [SMTPat (slice (append s1 s2) n1 n2)]
+let slice_append_suffix #a s1 s2 n1 n2 =
+  lemma_eq_intro (slice (append s1 s2) n1 n2) s2
+
+val slice_append_prefix: #a:Type -> s1:seq a -> s2:seq a ->
+  n1:nat{n1 == length s1} ->
+  Lemma (slice (append s1 s2) 0 n1 == s1)
+  [SMTPat (slice (append s1 s2) 0 n1)]
+let slice_append_prefix #a s1 s2 n1 =
+  lemma_eq_intro (slice (append s1 s2) 0 n1) s1
+
+let parse_u16_array_inv (len:U16.t) (b:bytes{length b == U16.v len}) :
+    Lemma (parse_u16_array (encode_u16_array len b) == Some ((len, b), 2 + U16.v len))
+    [SMTPat (parse_u16_array (encode_u16_array len b))] =
+  assert (length (encode_u16_array len b) == 2 + U16.v len);
+  assert (Some? (parse_u16_array (encode_u16_array len b)));
+  ()
+
+let parse_u32_array_inv (len:U32.t) (b:bytes{length b == U32.v len}) :
+    Lemma (parse_u32_array (encode_u32_array len b) == Some ((len, b), 4 + U32.v len))
+    [SMTPat (parse_u32_array (encode_u32_array len b))] =
+    assert (length (encode_u32_array len b) == 4 + U32.v len);
+    assert (Some? (parse_u32_array (encode_u32_array len b)));
+    ()
+
+// TODO: we're in trouble here - we have to argue that the sequential parsing
+// can be broken down into parsing appends (which is where the lack of lookahead
+// is important)
+let encode_entry_inverse (e:encoded_entry) :
+  Lemma (parse_entry (encode_entry e) == Some (e, length (encode_entry e))) =
+  // assert (Some? (parse_entry (encode_entry e)));
+  admit()
+
+val encode: store -> bytes
+let encode s = u32_to_be s.num_entries `append`
+               (List.fold_left (fun b e -> b `append` encode_entry e)
+               createEmpty s.entries)
+
 (*! Validating input buffer *)
 
 (** like a parser, a validator returns the number of bytes consumed *)
